examples/unit-tests/test_prims.fst
@@ -1,5 +1,5 @@
 (*
-   Copyright 2008-2014 Nikhil Swamy and Microsoft Research
+   Copyright 2008-2016 Nikhil Swamy and Microsoft Research
 
    Licensed under the Apache License, Version 2.0 (the "License");
    you may not use this file except in compliance with the License.
@@ -19,44 +19,59 @@ type False =
 
 (* True is the singleton inductive type *)
 type True =  
-  | T
+  | T      
 
-(* infix binary '=='; heterogeneous equality *)
-type Eq2 : #a:Type -> #b:Type -> a -> b -> Type  
+(* another singleton type, with its only inhabitant written '()'
+   we assume it as primitive, for convenient interop with other languages *)
+assume fresh type unit 
 
-(* booleans are primitive (TODO: make them inductives also) *)
-assume (* fresh *) type bool 
+(* infix binary '=='; heterogeneous equality; primitive (TODO: make it an inductive?) *)
+assume type Eq2 : #a:Type -> #b:Type -> a -> b -> Type  
+
+type bool = 
+ | B_true    //just 'true' in concrete syntax
+ | B_false   //just 'false in concrete syntax
+
+(* A proof irrelevant coercion to Type0: Elaborated in FStar.Squash.fst *)
+assume type squash : Type -> Type0 
 
 (* bool-to-type coercion *)
 opaque type b2t (b:bool) = (b == true) 
 
-(* infix binary '==>' *)
-opaque type l_imp (p:Type) (q:Type) = p -> Tot q                 
-                                          (* NB: The Tot effect is primitive; elaborated using PURE a few lines below *) 
-(* infix binary '/\' *) 
-type l_and  (p:Type) (q:Type) = 
-  | And   : p -> q -> (p /\ q)                                     
+(* constructive conjunction *)
+type c_and  (p:Type) (q:Type) = 
+  | And   : p -> q -> c_and p q
 
-(* infix binary '\/' *)
-type l_or   (p:Type) (q:Type) =                                  
-  | Left  : p -> (p \/ q)
-  | Right : q -> (p \/ q)
+(* '/\'  : specialized to Type#0 *)
+opaque type l_and (p:Type0) (q:Type0) = c_and p q
 
+(* constructive disjunction *)
+type c_or   (p:Type) (q:Type) =                                  
+  | Left  : p -> c_or p q
+  | Right : q -> c_or p q
+
+(* '\/'  : specialized to Type#0 *)
+opaque type l_or (p:Type0) (q:Type0) = c_or p q
+
+(* '==>' : specialized to Type#0 *)
+opaque type l_imp (p:Type0) (q:Type0) = p -> Tot q                 
+                                         (* ^^^ NB: The Tot effect is primitive;            *)
+				         (*         elaborated using PURE a few lines below *) 
 (* infix binary '<==>' *)
 opaque type l_iff (p:Type) (q:Type) = (p ==> q) /\ (q ==> p)       
 
 (* prefix unary '~' *)
 opaque type l_not (p:Type) = p ==> False                              
 
-logic type XOR (p:Type) (q:Type) = (p \/ q) /\ ~(p /\ q)
+type XOR (p:Type) (q:Type) = (p \/ q) /\ ~(p /\ q)
 
 opaque type ITE (p:Type) (q:Type) (r:Type) = (p ==> q) /\ (~p ==> r) 
 
 (* infix binary '<<'; a built-in well-founded partial order over all terms *)
-type Precedes : #a:Type -> #b:Type -> a -> b -> Type                
+assume type Precedes : #a:Type -> #b:Type -> a -> b -> Type0                
 
-(* forall (x:a). p x *)
-opaque type Forall (#a:Type) (p:a -> Type) = x:a -> Tot (p x)      
+(* forall (x:a). p x : specialized to Type#0 *)
+opaque type Forall (#a:Type) (p:a -> Type0) = x:a -> Tot (p x)      
 
 (* dependent pairs, aka strong sums *)
 type DTuple2 (a:Type)
@@ -65,12 +80,12 @@ type DTuple2 (a:Type)
             -> _2:b _1
             -> DTuple2 a b
 
-(* exists (x:a). p x *)
-opaque type Exists (#a:Type) (p:a -> Type) = x:a & p x          
+(* exists (x:a). p x : specialized to Type#0 *)
+opaque type Exists (#a:Type) (p:a -> Type0) = x:a & p x          
 
 (* PURE effect *)
-type PurePre = Type
-type PurePost (a:Type) = a -> Type
+type PurePre = Type0
+type PurePost (a:Type) = a -> Type0
 type PureWP   (a:Type) = PurePost a -> Tot PurePre
 type pure_return (a:Type) (x:a) (p:PurePost a) =
      p x
@@ -95,461 +110,460 @@ type pure_wp_as_type (a:Type) (wp:PureWP a) = (forall (p:PurePost a). wp p)
 type pure_close_wp (a:Type) (b:Type) (wp:(b -> Tot (PureWP a))) (p:PurePost a) = (forall (b:b). wp b p)
 type pure_assert_p (a:Type) (q:Type) (wp:PureWP a) (p:PurePost a) = (q /\ wp p)
 type pure_assume_p (a:Type) (q:Type) (wp:PureWP a) (p:PurePost a) = (q ==> wp p)
-type pure_null_wp (a:Type) (p:PurePost a) = (forall (x:a). p x)
-type pure_trivial (a:Type) (wp:PureWP a) = wp (fun (x:a) -> True)
+type pure_null_wp  (a:Type) (p:PurePost a) = (forall (x:a). p x)
+type pure_trivial  (a:Type) (wp:PureWP a) = wp (fun (x:a) -> True)
 
-total new_effect { (* The definition of the PURE effect is fixed; no user should ever change this *)
-  PURE : a:Type -> wp:PureWP a -> wlp:PureWP a -> Effect
-  with return       = pure_return
-     ; bind_wlp     = pure_bind_wlp
-     ; bind_wp      = pure_bind_wp
-     ; if_then_else = pure_if_then_else
-     ; ite_wlp      = pure_ite_wlp
-     ; ite_wp       = pure_ite_wp
-     ; wp_binop     = pure_wp_binop
-     ; wp_as_type   = pure_wp_as_type
-     ; close_wp     = pure_close_wp
-     ; assert_p     = pure_assert_p
-     ; assume_p     = pure_assume_p
-     ; null_wp      = pure_null_wp
-     ; trivial      = pure_trivial
-}
+// total new_effect { (* The definition of the PURE effect is fixed; no user should ever change this *)
+//   PURE : a:Type -> wp:PureWP a -> wlp:PureWP a -> Effect
+//   with return       = pure_return
+//      ; bind_wlp     = pure_bind_wlp
+//      ; bind_wp      = pure_bind_wp
+//      ; if_then_else = pure_if_then_else
+//      ; ite_wlp      = pure_ite_wlp
+//      ; ite_wp       = pure_ite_wp
+//      ; wp_binop     = pure_wp_binop
+//      ; wp_as_type   = pure_wp_as_type
+//      ; close_wp     = pure_close_wp
+//      ; assert_p     = pure_assert_p
+//      ; assume_p     = pure_assume_p
+//      ; null_wp      = pure_null_wp
+//      ; trivial      = pure_trivial
+// }
 
-effect Pure (a:Type) (pre:PurePre) (post:PurePost a) =
-        PURE a
-             (fun (p:PurePost a) -> pre /\ (forall (x:a). post x ==> p x)) (* PureWP *)
-             (fun (p:PurePost a) -> forall (x:a). pre /\ post x ==> p x)   (* WLP *)
-effect Admit (a:Type) = PURE a (fun (p:PurePost a) -> True) (fun (p:PurePost a) -> True)
-default effect Tot (a:Type) = PURE a (pure_null_wp a) (pure_null_wp a)
+// // effect Pure (a:Type) (pre:PurePre) (post:PurePost a) =
+// //         PURE a
+// //              (fun (p:PurePost a) -> pre /\ (forall (x:a). post x ==> p x)) (* PureWP *)
+// //              (fun (p:PurePost a) -> forall (x:a). pre /\ post x ==> p x)   (* WLP *)
+// // effect Admit (a:Type) = PURE a (fun (p:PurePost a) -> True) (fun (p:PurePost a) -> True)
+// // default effect Tot (a:Type) = PURE a (pure_null_wp a) (pure_null_wp a)
 
-total new_effect GHOST = PURE
-sub_effect
-  PURE ~> GHOST = fun (a:Type) (wp:PureWP a) -> wp
-default effect GTot (a:Type) = GHOST a (pure_null_wp a) (pure_null_wp a)
-effect Ghost (a:Type) (pre:Type) (post:PurePost a) =
-       GHOST a
-           (fun (p:PurePost a) -> pre /\ (forall (x:a). post x ==> p x))
-           (fun (p:PurePost a) -> forall (x:a). pre /\ post x ==> p x)
+// // total new_effect GHOST = PURE
+// // sub_effect
+// //   PURE ~> GHOST = fun (a:Type) (wp:PureWP a) -> wp
+// // default effect GTot (a:Type) = GHOST a (pure_null_wp a) (pure_null_wp a)
+// // effect Ghost (a:Type) (pre:Type) (post:PurePost a) =
+// //        GHOST a
+// //            (fun (p:PurePost a) -> pre /\ (forall (x:a). post x ==> p x))
+// //            (fun (p:PurePost a) -> forall (x:a). pre /\ post x ==> p x)
 
-type unit
-type int
-assume val op_AmpAmp             : bool -> bool -> Tot bool
-assume val op_BarBar             : bool -> bool -> Tot bool
-assume val op_Negation           : bool -> Tot bool
-assume val op_Multiply           : int -> int -> Tot int
-assume val op_Subtraction        : int -> int -> Tot int
-assume val op_Addition           : int -> int -> Tot int
-assume val op_Minus              : int -> Tot int
-assume val op_LessThanOrEqual    : int -> int -> Tot bool
-assume val op_GreaterThan        : int -> int -> Tot bool
-assume val op_GreaterThanOrEqual : int -> int -> Tot bool
-assume val op_LessThan           : int -> int -> Tot bool
-(* Primitive (structural) equality.
-   What about for function types? *)
-assume val op_Equality :    #a:Type -> a -> a -> Tot bool
-assume val op_disEquality : #a:Type -> a -> a -> Tot bool
+// // assume fresh type unit
+// // assume fresh type int
+// // assume val op_AmpAmp             : bool -> bool -> Tot bool
+// // assume val op_BarBar             : bool -> bool -> Tot bool
+// // assume val op_Negation           : bool -> Tot bool
+// // assume val op_Multiply           : int -> int -> Tot int
+// // assume val op_Subtraction        : int -> int -> Tot int
+// // assume val op_Addition           : int -> int -> Tot int
+// // assume val op_Minus              : int -> Tot int
+// // assume val op_LessThanOrEqual    : int -> int -> Tot bool
+// // assume val op_GreaterThan        : int -> int -> Tot bool
+// // assume val op_GreaterThanOrEqual : int -> int -> Tot bool
+// // assume val op_LessThan           : int -> int -> Tot bool
+// // (* Primitive (structural) equality.
+// //    What about for function types? *)
+// // assume val op_Equality :    #a:Type -> a -> a -> Tot bool
+// // assume val op_disEquality : #a:Type -> a -> a -> Tot bool
 
-(* type int16 = i:int{i > -32769 /\ 32768 > i} *)
-type int32 = int
-type int64
-type uint8
-type uint16
-type uint32
-type uint64
-type char
-type float
-type string
-type array : Type -> Type
-assume val strcat : string -> string -> Tot string
-type exn
-type HashMultiMap : Type -> Type -> Type //needed for bootstrapping
-type byte = uint8
-type double = float
+// // (* type int16 = i:int{i > -32769 /\ 32768 > i} *)
+// // type int32 = int
+// // assume fresh type int64
+// // assume fresh type uint8
+// // assume fresh type uint16
+// // assume fresh type uint32
+// // assume fresh type uint64
+// // assume fresh type char
+// // assume fresh type float
+// // assume fresh type string
+// // ??type array : Type -> Type 
+// // assume val strcat : string -> string -> Tot string
+// // assume fresh type exn
+// // type HashMultiMap : Type -> Type -> Type //needed for bootstrapping
+// // type byte = uint8
+// // type double = float
 
-type list (a:Type) =
-  | Nil  : list a
-  | Cons : hd:a -> tl:list a -> list a
+// // type list (a:Type) =
+// //   | Nil  : list a
+// //   | Cons : hd:a -> tl:list a -> list a
 
-type pattern =
-  | SMTPat   : #a:Type -> a -> pattern
-  | SMTPatT  : a:Type -> pattern
-  | SMTPatOr : list (list pattern) -> pattern
+// // type pattern =
+// //   | SMTPat   : #a:Type -> a -> pattern
+// //   | SMTPatT  : a:Type -> pattern
+// //   | SMTPatOr : list (list pattern) -> pattern
 
-assume type decreases : #a:Type -> a -> Type
+// // assume type decreases : #a:Type -> a -> Type
 
-effect Lemma (a:Type) (pre:Type) (post:Type) (pats:list pattern) =
-       Pure a pre (fun r -> post)
+// // effect Lemma (a:Type) (pre:Type) (post:Type) (pats:list pattern) =
+// //        Pure a pre (fun r -> post)
 
-(*
-   Lemma is desugared specially. You can write:
+// // (*
+// //    Lemma is desugared specially. You can write:
 
-     Lemma phi                 for   Lemma (requires True) phi []
-     Lemma t1..tn              for   Lemma unit t1..tn
-*)
-type option (a:Type) =
-  | None : option a
-  | Some : v:a -> option a
+// //      Lemma phi                 for   Lemma (requires True) phi []
+// //      Lemma t1..tn              for   Lemma unit t1..tn
+// // *)
+// // type option (a:Type) =
+// //   | None : option a
+// //   | Some : v:a -> option a
 
-type either 'a 'b =
-  | Inl : v:'a -> either 'a 'b
-  | Inr : v:'b -> either 'a 'b
+// // type either 'a 'b =
+// //   | Inl : v:'a -> either 'a 'b
+// //   | Inr : v:'b -> either 'a 'b
 
-type result (a:Type) =
-  | V   : v:a -> result a
-  | E   : e:exn -> result a
-  | Err : msg:string -> result a
+// // type result (a:Type) =
+// //   | V   : v:a -> result a
+// //   | E   : e:exn -> result a
+// //   | Err : msg:string -> result a
 
-new_effect DIV = PURE
-effect Div (a:Type) (pre:PurePre) (post:PurePost a) =
-       DIV a
-           (fun (p:PurePost a) -> pre /\ (forall a. post a ==> p a)) (* WP *)
-           (fun (p:PurePost a) -> forall a. pre /\ post a ==> p a)   (* WLP *)
+// // new_effect DIV = PURE
+// // effect Div (a:Type) (pre:PurePre) (post:PurePost a) =
+// //        DIV a
+// //            (fun (p:PurePost a) -> pre /\ (forall a. post a ==> p a)) (* WP *)
+// //            (fun (p:PurePost a) -> forall a. pre /\ post a ==> p a)   (* WLP *)
 
-default effect Dv (a:Type) =
-     DIV a (fun (p:PurePost a) -> (forall (x:a). p x))
-           (fun (p:PurePost a) -> (forall (x:a). p x))
+// // default effect Dv (a:Type) =
+// //      DIV a (fun (p:PurePost a) -> (forall (x:a). p x))
+// //            (fun (p:PurePost a) -> (forall (x:a). p x))
 
-type STPre_h  (heap:Type)          = heap -> Type
-type STPost_h (heap:Type) (a:Type) = a -> heap -> Type
-type STWP_h   (heap:Type) (a:Type) = STPost_h heap a -> Tot (STPre_h heap)
+// // type STPre_h  (heap:Type)          = heap -> Type
+// // type STPost_h (heap:Type) (a:Type) = a -> heap -> Type
+// // type STWP_h   (heap:Type) (a:Type) = STPost_h heap a -> Tot (STPre_h heap)
 
-type st_return        (heap:Type) (a:Type)
-                      (x:a) (p:STPost_h heap a) =
-     p x
-type st_bind_wp       (heap:Type) (a:Type) (b:Type)
-                      (wp1:STWP_h heap a) (wlp1:STWP_h heap a)
-                      (wp2:(a -> Tot (STWP_h heap b))) (wlp2:(a -> Tot (STWP_h heap b)))
-                      (p:STPost_h heap b) (h0:heap) =
-     wp1 (fun a -> wp2 a p) h0
-type st_bind_wlp      (heap:Type) (a:Type) (b:Type)
-                      (wlp1:STWP_h heap a) (wlp2:(a -> Tot (STWP_h heap b)))
-                      (p:STPost_h heap b) (h0:heap) =
-     wlp1 (fun a -> wlp2 a p) h0
-type st_if_then_else  (heap:Type) (a:Type) (p:Type)
-                      (wp_then:STWP_h heap a) (wp_else:STWP_h heap a)
-                      (post:STPost_h heap a) (h0:heap) =
-     ITE p
-        (wp_then post h0)
-	(wp_else post h0)
-type st_ite_wlp       (heap:Type) (a:Type)
-                      (wlp_cases:STWP_h heap a)
-                      (post:STPost_h heap a) (h0:heap) =
-     (forall (a:a) (h:heap).
-           wlp_cases (fun a1 h1 -> a=!=a1 \/ h=!=h1) h0
-        \/ post a h)
-type st_ite_wp        (heap:Type) (a:Type)
-                      (wlp_cases:STWP_h heap a) (wp_cases:STWP_h heap a)
-                      (post:STPost_h heap a) (h0:heap) =
-     st_ite_wlp heap a wlp_cases post h0
-     /\ wp_cases (fun a h_ -> True) h0
-type st_wp_binop      (heap:Type) (a:Type)
-                      (wp1:STWP_h heap a)
-                      (op:(Type -> Type -> Type))
-                      (wp2:STWP_h heap a)
-                      (p:STPost_h heap a) (h:heap) =
-     op (wp1 p h) (wp2 p h)
-type st_wp_as_type    (heap:Type) (a:Type) (wp:STWP_h heap a) =
-     (forall (p:STPost_h heap a) (h:heap). wp p h)
-type st_close_wp      (heap:Type) (a:Type) (b:Type)
-                      (wp:(b -> Tot (STWP_h heap a)))
-                      (p:STPost_h heap a) (h:heap) =
-     (forall (b:b). wp b p h)
-type st_assert_p      (heap:Type) (a:Type) (p:Type)
-                      (wp:STWP_h heap a)
-                      (q:STPost_h heap a) (h:heap) =
-     p /\ wp q h
-type st_assume_p      (heap:Type) (a:Type) (p:Type)
-                      (wp:STWP_h heap a)
-                      (q:STPost_h heap a) (h:heap) =
-     p ==> wp q h
-type st_null_wp       (heap:Type) (a:Type)
-                      (p:STPost_h heap a) (h:heap) =
-     (forall (x:a) (h:heap). p x h)
-type st_trivial       (heap:Type) (a:Type)
-                      (wp:STWP_h heap a) =
-     (forall h0. wp (fun r h1 -> True) h0)
+// // type st_return        (heap:Type) (a:Type)
+// //                       (x:a) (p:STPost_h heap a) =
+// //      p x
+// // type st_bind_wp       (heap:Type) (a:Type) (b:Type)
+// //                       (wp1:STWP_h heap a) (wlp1:STWP_h heap a)
+// //                       (wp2:(a -> Tot (STWP_h heap b))) (wlp2:(a -> Tot (STWP_h heap b)))
+// //                       (p:STPost_h heap b) (h0:heap) =
+// //      wp1 (fun a -> wp2 a p) h0
+// // type st_bind_wlp      (heap:Type) (a:Type) (b:Type)
+// //                       (wlp1:STWP_h heap a) (wlp2:(a -> Tot (STWP_h heap b)))
+// //                       (p:STPost_h heap b) (h0:heap) =
+// //      wlp1 (fun a -> wlp2 a p) h0
+// // type st_if_then_else  (heap:Type) (a:Type) (p:Type)
+// //                       (wp_then:STWP_h heap a) (wp_else:STWP_h heap a)
+// //                       (post:STPost_h heap a) (h0:heap) =
+// //      ITE p
+// //         (wp_then post h0)
+// // 	(wp_else post h0)
+// // type st_ite_wlp       (heap:Type) (a:Type)
+// //                       (wlp_cases:STWP_h heap a)
+// //                       (post:STPost_h heap a) (h0:heap) =
+// //      (forall (a:a) (h:heap).
+// //            wlp_cases (fun a1 h1 -> a=!=a1 \/ h=!=h1) h0
+// //         \/ post a h)
+// // type st_ite_wp        (heap:Type) (a:Type)
+// //                       (wlp_cases:STWP_h heap a) (wp_cases:STWP_h heap a)
+// //                       (post:STPost_h heap a) (h0:heap) =
+// //      st_ite_wlp heap a wlp_cases post h0
+// //      /\ wp_cases (fun a h_ -> True) h0
+// // type st_wp_binop      (heap:Type) (a:Type)
+// //                       (wp1:STWP_h heap a)
+// //                       (op:(Type -> Type -> Type))
+// //                       (wp2:STWP_h heap a)
+// //                       (p:STPost_h heap a) (h:heap) =
+// //      op (wp1 p h) (wp2 p h)
+// // type st_wp_as_type    (heap:Type) (a:Type) (wp:STWP_h heap a) =
+// //      (forall (p:STPost_h heap a) (h:heap). wp p h)
+// // type st_close_wp      (heap:Type) (a:Type) (b:Type)
+// //                       (wp:(b -> Tot (STWP_h heap a)))
+// //                       (p:STPost_h heap a) (h:heap) =
+// //      (forall (b:b). wp b p h)
+// // type st_assert_p      (heap:Type) (a:Type) (p:Type)
+// //                       (wp:STWP_h heap a)
+// //                       (q:STPost_h heap a) (h:heap) =
+// //      p /\ wp q h
+// // type st_assume_p      (heap:Type) (a:Type) (p:Type)
+// //                       (wp:STWP_h heap a)
+// //                       (q:STPost_h heap a) (h:heap) =
+// //      p ==> wp q h
+// // type st_null_wp       (heap:Type) (a:Type)
+// //                       (p:STPost_h heap a) (h:heap) =
+// //      (forall (x:a) (h:heap). p x h)
+// // type st_trivial       (heap:Type) (a:Type)
+// //                       (wp:STWP_h heap a) =
+// //      (forall h0. wp (fun r h1 -> True) h0)
 
-new_effect {
-  STATE_h (heap:Type) : result:Type -> wp:STWP_h heap result -> wlp:STWP_h heap result -> Effect
-  with return       = st_return heap
-     ; bind_wp      = st_bind_wp heap
-     ; bind_wlp     = st_bind_wlp heap
-     ; if_then_else = st_if_then_else heap
-     ; ite_wlp      = st_ite_wlp heap
-     ; ite_wp       = st_ite_wp heap
-     ; wp_binop     = st_wp_binop heap
-     ; wp_as_type   = st_wp_as_type heap
-     ; close_wp     = st_close_wp heap
-     ; assert_p     = st_assert_p heap
-     ; assume_p     = st_assume_p heap
-     ; null_wp      = st_null_wp heap
-     ; trivial      = st_trivial heap
-}
+// // // new_effect {
+// // //   STATE_h (heap:Type) : result:Type -> wp:STWP_h heap result -> wlp:STWP_h heap result -> Effect
+// // //   with return       = st_return heap
+// // //      ; bind_wp      = st_bind_wp heap
+// // //      ; bind_wlp     = st_bind_wlp heap
+// // //      ; if_then_else = st_if_then_else heap
+// // //      ; ite_wlp      = st_ite_wlp heap
+// // //      ; ite_wp       = st_ite_wp heap
+// // //      ; wp_binop     = st_wp_binop heap
+// // //      ; wp_as_type   = st_wp_as_type heap
+// // //      ; close_wp     = st_close_wp heap
+// // //      ; assert_p     = st_assert_p heap
+// // //      ; assume_p     = st_assume_p heap
+// // //      ; null_wp      = st_null_wp heap
+// // //      ; trivial      = st_trivial heap
+// // // }
 
-(* Effect EXCEPTION *)
-type ExPre  = Type
-type ExPost (a:Type) = result a -> Type
-type ExWP   (a:Type) = ExPost a -> Tot ExPre
-type ex_return (a:Type) (x:a) (p:ExPost a) = p (V x)
-type ex_bind_wlp (a:Type) (b:Type) (wlp1:ExWP a) (wlp2:(a -> Tot (ExWP b))) (p:ExPost b) =
-   (forall (rb:result b). p rb \/ wlp1 (fun ra1 -> ITE (b2t (is_V ra1))
-                                              (wlp2 (V.v ra1) (fun rb2 -> rb2=!=rb))
-                                              (ra1 =!= rb)))
-type ex_bind_wp (a:Type) (b:Type) 
-		(wp1:ExWP a) (wlp1:ExWP a) 
-		(wp2:(a -> Tot (ExWP b))) (wlp2:(a -> Tot (ExWP b))) (p:ExPost b) =
-   ex_bind_wlp a b wlp1 wlp2 p
-   /\ wp1 (fun ra1 -> (ITE (b2t (is_V ra1))
-                            (wp2 (V.v ra1) (fun rb2 -> True))
-                             True))
-type ex_if_then_else (a:Type) (p:Type) (wp_then:ExWP a) (wp_else:ExWP a) (post:ExPost a) =
-   ITE p
-       (wp_then post)
-       (wp_else post)
-type ex_ite_wlp  (a:Type) (wlp_cases:ExWP a) (post:ExPost a) =
-    (forall (a:result a). wlp_cases (fun a1 -> a=!=a1) \/ post a)
-type ex_ite_wp (a:Type) (wlp_cases:ExWP a) (wp_cases:ExWP a) (post:ExPost a) =
-    ex_ite_wlp a wlp_cases post
-    /\ wp_cases (fun ra2 -> True)
-type ex_wp_binop (a:Type) (wp1:ExWP a) (op:(Type -> Type -> Type)) (wp2:ExWP a) (p:ExPost a) =
-   op (wp1 p) (wp2 p)
-type ex_wp_as_type (a:Type) (wp:ExWP a) = (forall (p:ExPost a). wp p)
-type ex_close_wp (a:Type) (b:Type) (wp:(b -> Tot (ExWP a))) (p:ExPost a) = (forall (b:b). wp b p)
-type ex_assert_p (a:Type) (q:Type) (wp:ExWP a) (p:ExPost a) = (q /\ wp p)
-type ex_assume_p (a:Type) (q:Type) (wp:ExWP a) (p:ExPost a) = (q ==> wp p)
-type ex_null_wp (a:Type) (p:ExPost a) = (forall (r:result a). p r)
-type ex_trivial (a:Type) (wp:ExWP a) = wp (fun r -> True)
+// // // (* Effect EXCEPTION *)
+// // // type ExPre  = Type
+// // // type ExPost (a:Type) = result a -> Type
+// // // type ExWP   (a:Type) = ExPost a -> Tot ExPre
+// // // type ex_return (a:Type) (x:a) (p:ExPost a) = p (V x)
+// // // type ex_bind_wlp (a:Type) (b:Type) (wlp1:ExWP a) (wlp2:(a -> Tot (ExWP b))) (p:ExPost b) =
+// // //    (forall (rb:result b). p rb \/ wlp1 (fun ra1 -> ITE (b2t (is_V ra1))
+// // //                                               (wlp2 (V.v ra1) (fun rb2 -> rb2=!=rb))
+// // //                                               (ra1 =!= rb)))
+// // // type ex_bind_wp (a:Type) (b:Type) 
+// // // 		(wp1:ExWP a) (wlp1:ExWP a) 
+// // // 		(wp2:(a -> Tot (ExWP b))) (wlp2:(a -> Tot (ExWP b))) (p:ExPost b) =
+// // //    ex_bind_wlp a b wlp1 wlp2 p
+// // //    /\ wp1 (fun ra1 -> (ITE (b2t (is_V ra1))
+// // //                             (wp2 (V.v ra1) (fun rb2 -> True))
+// // //                              True))
+// // // type ex_if_then_else (a:Type) (p:Type) (wp_then:ExWP a) (wp_else:ExWP a) (post:ExPost a) =
+// // //    ITE p
+// // //        (wp_then post)
+// // //        (wp_else post)
+// // // type ex_ite_wlp  (a:Type) (wlp_cases:ExWP a) (post:ExPost a) =
+// // //     (forall (a:result a). wlp_cases (fun a1 -> a=!=a1) \/ post a)
+// // // type ex_ite_wp (a:Type) (wlp_cases:ExWP a) (wp_cases:ExWP a) (post:ExPost a) =
+// // //     ex_ite_wlp a wlp_cases post
+// // //     /\ wp_cases (fun ra2 -> True)
+// // // type ex_wp_binop (a:Type) (wp1:ExWP a) (op:(Type -> Type -> Type)) (wp2:ExWP a) (p:ExPost a) =
+// // //    op (wp1 p) (wp2 p)
+// // // type ex_wp_as_type (a:Type) (wp:ExWP a) = (forall (p:ExPost a). wp p)
+// // // type ex_close_wp (a:Type) (b:Type) (wp:(b -> Tot (ExWP a))) (p:ExPost a) = (forall (b:b). wp b p)
+// // // type ex_assert_p (a:Type) (q:Type) (wp:ExWP a) (p:ExPost a) = (q /\ wp p)
+// // // type ex_assume_p (a:Type) (q:Type) (wp:ExWP a) (p:ExPost a) = (q ==> wp p)
+// // // type ex_null_wp (a:Type) (p:ExPost a) = (forall (r:result a). p r)
+// // // type ex_trivial (a:Type) (wp:ExWP a) = wp (fun r -> True)
 
-new_effect {
-  EXN : result:Type -> wp:ExWP result -> wlp:ExWP result -> Effect
-  with
-    return       = ex_return
-  ; bind_wlp     = ex_bind_wlp
-  ; bind_wp      = ex_bind_wp
-  ; if_then_else = ex_if_then_else
-  ; ite_wlp      = ex_ite_wlp
-  ; ite_wp       = ex_ite_wp
-  ; wp_binop     = ex_wp_binop
-  ; wp_as_type   = ex_wp_as_type
-  ; close_wp     = ex_close_wp
-  ; assert_p     = ex_assert_p
-  ; assume_p     = ex_assume_p
-  ; null_wp      = ex_null_wp
-  ; trivial      = ex_trivial
-}
-effect Exn (a:Type) (pre:ExPre) (post:ExPost a) =
-       EXN a
-         (fun (p:ExPost a) -> pre /\ (forall (r:result a). (pre /\ post r) ==> p r)) (* WP *)
-         (fun (p:ExPost a) -> (forall (r:result a). (pre /\ post r) ==> p r))       (* WLP *)
-default effect Ex (a:Type) = Exn a True (fun v -> True)
+// // // new_effect {
+// // //   EXN : result:Type -> wp:ExWP result -> wlp:ExWP result -> Effect
+// // //   with
+// // //     return       = ex_return
+// // //   ; bind_wlp     = ex_bind_wlp
+// // //   ; bind_wp      = ex_bind_wp
+// // //   ; if_then_else = ex_if_then_else
+// // //   ; ite_wlp      = ex_ite_wlp
+// // //   ; ite_wp       = ex_ite_wp
+// // //   ; wp_binop     = ex_wp_binop
+// // //   ; wp_as_type   = ex_wp_as_type
+// // //   ; close_wp     = ex_close_wp
+// // //   ; assert_p     = ex_assert_p
+// // //   ; assume_p     = ex_assume_p
+// // //   ; null_wp      = ex_null_wp
+// // //   ; trivial      = ex_trivial
+// // // }
+// // // effect Exn (a:Type) (pre:ExPre) (post:ExPost a) =
+// // //        EXN a
+// // //          (fun (p:ExPost a) -> pre /\ (forall (r:result a). (pre /\ post r) ==> p r)) (* WP *)
+// // //          (fun (p:ExPost a) -> (forall (r:result a). (pre /\ post r) ==> p r))       (* WLP *)
+// // // default effect Ex (a:Type) = Exn a True (fun v -> True)
 
-type AllPre_h  (h:Type)           = h -> Type
-type AllPost_h (h:Type) (a:Type)  = result a -> h -> Type
-type AllWP_h   (h:Type) (a:Type)  = AllPost_h h a -> Tot (AllPre_h h)
+// // // type AllPre_h  (h:Type)           = h -> Type
+// // // type AllPost_h (h:Type) (a:Type)  = result a -> h -> Type
+// // // type AllWP_h   (h:Type) (a:Type)  = AllPost_h h a -> Tot (AllPre_h h)
 
-type all_return  (heap:Type) (a:Type) (x:a) (p:AllPost_h heap a) = p (V x)
-type all_bind_wp (heap:Type) (a:Type) (b:Type)
-                 (wp1:AllWP_h heap a) (wlp1:AllWP_h heap a)
-                 (wp2:(a -> Tot (AllWP_h heap b))) (wlp2:(a -> Tot (AllWP_h heap b)))
-                 (p:AllPost_h heap b) (h0:heap) =
-   (wp1 (fun ra h1 -> b2t(is_V ra) ==> wp2 (V.v ra) p h1) h0)
-type all_bind_wlp (heap:Type) (a:Type) (b:Type)
-                  (wlp1:AllWP_h heap a) (wlp2:(a -> Tot (AllWP_h heap b)))
-                  (p:AllPost_h heap b) (h0:heap) =
-   (forall rb h. wlp1 (fun ra h1 ->
-       ITE (b2t (is_V ra))
-           (wlp2 (V.v ra) (fun rb2 h2 -> rb=!=rb2 \/ h=!=h2) h1)
-           (rb=!=ra \/ h=!=h1)) h0 \/ p rb h)
-type all_if_then_else (heap:Type) (a:Type) (p:Type)
-                      (wp_then:AllWP_h heap a) (wp_else:AllWP_h heap a)
-                      (post:AllPost_h heap a) (h0:heap) =
-   ITE p
-       (wp_then post h0)
-       (wp_else post h0)
-type all_ite_wlp  (heap:Type) (a:Type)
-                  (wlp_cases:AllWP_h heap a)
-                  (post:AllPost_h heap a) (h0:heap) =
-     (forall (ra:result a) (h:heap). wlp_cases (fun ra2 h2 -> ra=!=ra2 \/ h=!=h2) h0 \/ post ra h)
-type all_ite_wp (heap:Type) (a:Type)
-                (wlp_cases:AllWP_h heap a) (wp_cases:AllWP_h heap a)
-                (post:AllPost_h heap a) (h0:heap) =
-     (forall (ra:result a) (h:heap). wlp_cases (fun ra2 h2 -> ra=!=ra2 \/ h=!=h2) h0 \/ post ra h)
-      /\ wp_cases (fun _a _b -> True) h0
-type all_wp_binop (heap:Type) (a:Type)
-                  (wp1:AllWP_h heap a) (op:(Type -> Type -> Type))
-                  (wp2:AllWP_h heap a) (p:AllPost_h heap a) (h:heap) =
-     op (wp1 p h) (wp2 p h)
-type all_wp_as_type (heap:Type) (a:Type) (wp:AllWP_h heap a) =
-    (forall (p:AllPost_h heap a) (h:heap). wp p h)
-type all_close_wp (heap:Type) (a:Type) (b:Type)
-                  (wp:(b -> Tot (AllWP_h heap a)))
-                  (p:AllPost_h heap a) (h:heap) =
-    (forall (b:b). wp b p h)
-type all_assert_p (heap:Type) (a:Type) (p:Type)
-                  (wp:AllWP_h heap a) (q:AllPost_h heap a) (h:heap) =
-    p /\ wp q h
-type all_assume_p (heap:Type) (a:Type) (p:Type)
-                  (wp:AllWP_h heap a) (q:AllPost_h heap a) (h:heap) =
-    p ==> wp q h
-type all_null_wp (heap:Type) (a:Type)
-                 (p:AllPost_h heap a) (h0:heap) =
-    (forall (a:result a) (h:heap). p a h)
-type all_trivial (heap:Type) (a:Type) (wp:AllWP_h heap a) =
-    (forall (h0:heap). wp (fun r h1 -> True) h0)
+// // // type all_return  (heap:Type) (a:Type) (x:a) (p:AllPost_h heap a) = p (V x)
+// // // type all_bind_wp (heap:Type) (a:Type) (b:Type)
+// // //                  (wp1:AllWP_h heap a) (wlp1:AllWP_h heap a)
+// // //                  (wp2:(a -> Tot (AllWP_h heap b))) (wlp2:(a -> Tot (AllWP_h heap b)))
+// // //                  (p:AllPost_h heap b) (h0:heap) =
+// // //    (wp1 (fun ra h1 -> b2t(is_V ra) ==> wp2 (V.v ra) p h1) h0)
+// // // type all_bind_wlp (heap:Type) (a:Type) (b:Type)
+// // //                   (wlp1:AllWP_h heap a) (wlp2:(a -> Tot (AllWP_h heap b)))
+// // //                   (p:AllPost_h heap b) (h0:heap) =
+// // //    (forall rb h. wlp1 (fun ra h1 ->
+// // //        ITE (b2t (is_V ra))
+// // //            (wlp2 (V.v ra) (fun rb2 h2 -> rb=!=rb2 \/ h=!=h2) h1)
+// // //            (rb=!=ra \/ h=!=h1)) h0 \/ p rb h)
+// // // type all_if_then_else (heap:Type) (a:Type) (p:Type)
+// // //                       (wp_then:AllWP_h heap a) (wp_else:AllWP_h heap a)
+// // //                       (post:AllPost_h heap a) (h0:heap) =
+// // //    ITE p
+// // //        (wp_then post h0)
+// // //        (wp_else post h0)
+// // // type all_ite_wlp  (heap:Type) (a:Type)
+// // //                   (wlp_cases:AllWP_h heap a)
+// // //                   (post:AllPost_h heap a) (h0:heap) =
+// // //      (forall (ra:result a) (h:heap). wlp_cases (fun ra2 h2 -> ra=!=ra2 \/ h=!=h2) h0 \/ post ra h)
+// // // type all_ite_wp (heap:Type) (a:Type)
+// // //                 (wlp_cases:AllWP_h heap a) (wp_cases:AllWP_h heap a)
+// // //                 (post:AllPost_h heap a) (h0:heap) =
+// // //      (forall (ra:result a) (h:heap). wlp_cases (fun ra2 h2 -> ra=!=ra2 \/ h=!=h2) h0 \/ post ra h)
+// // //       /\ wp_cases (fun _a _b -> True) h0
+// // // type all_wp_binop (heap:Type) (a:Type)
+// // //                   (wp1:AllWP_h heap a) (op:(Type -> Type -> Type))
+// // //                   (wp2:AllWP_h heap a) (p:AllPost_h heap a) (h:heap) =
+// // //      op (wp1 p h) (wp2 p h)
+// // // type all_wp_as_type (heap:Type) (a:Type) (wp:AllWP_h heap a) =
+// // //     (forall (p:AllPost_h heap a) (h:heap). wp p h)
+// // // type all_close_wp (heap:Type) (a:Type) (b:Type)
+// // //                   (wp:(b -> Tot (AllWP_h heap a)))
+// // //                   (p:AllPost_h heap a) (h:heap) =
+// // //     (forall (b:b). wp b p h)
+// // // type all_assert_p (heap:Type) (a:Type) (p:Type)
+// // //                   (wp:AllWP_h heap a) (q:AllPost_h heap a) (h:heap) =
+// // //     p /\ wp q h
+// // // type all_assume_p (heap:Type) (a:Type) (p:Type)
+// // //                   (wp:AllWP_h heap a) (q:AllPost_h heap a) (h:heap) =
+// // //     p ==> wp q h
+// // // type all_null_wp (heap:Type) (a:Type)
+// // //                  (p:AllPost_h heap a) (h0:heap) =
+// // //     (forall (a:result a) (h:heap). p a h)
+// // // type all_trivial (heap:Type) (a:Type) (wp:AllWP_h heap a) =
+// // //     (forall (h0:heap). wp (fun r h1 -> True) h0)
 
-new_effect {
-  ALL_h (heap:Type) : a:Type -> wp:AllWP_h heap a -> wlp:AllWP_h heap a -> Effect
-  with
-    return       = all_return       heap
-  ; bind_wp      = all_bind_wp      heap
-  ; bind_wlp     = all_bind_wlp     heap
-  ; if_then_else = all_if_then_else heap
-  ; ite_wlp      = all_ite_wlp      heap
-  ; ite_wp       = all_ite_wp       heap
-  ; wp_binop     = all_wp_binop     heap
-  ; wp_as_type   = all_wp_as_type   heap
-  ; close_wp     = all_close_wp     heap
-  ; assert_p     = all_assert_p     heap
-  ; assume_p     = all_assume_p     heap
-  ; null_wp      = all_null_wp      heap
-  ; trivial      = all_trivial      heap
-}
+// // // new_effect {
+// // //   ALL_h (heap:Type) : a:Type -> wp:AllWP_h heap a -> wlp:AllWP_h heap a -> Effect
+// // //   with
+// // //     return       = all_return       heap
+// // //   ; bind_wp      = all_bind_wp      heap
+// // //   ; bind_wlp     = all_bind_wlp     heap
+// // //   ; if_then_else = all_if_then_else heap
+// // //   ; ite_wlp      = all_ite_wlp      heap
+// // //   ; ite_wp       = all_ite_wp       heap
+// // //   ; wp_binop     = all_wp_binop     heap
+// // //   ; wp_as_type   = all_wp_as_type   heap
+// // //   ; close_wp     = all_close_wp     heap
+// // //   ; assert_p     = all_assert_p     heap
+// // //   ; assume_p     = all_assume_p     heap
+// // //   ; null_wp      = all_null_wp      heap
+// // //   ; trivial      = all_trivial      heap
+// // // }
 
-sub_effect
-  PURE  ~> DIV   = fun (a:Type) (wp:PureWP a) (p:PurePost a) -> wp (fun a -> p a)
-sub_effect
-  DIV   ~> EXN   = fun (a:Type) (wp:PureWP a) (p:ExPost a) -> wp (fun a -> p (V a))
+// // // sub_effect
+// // //   PURE  ~> DIV   = fun (a:Type) (wp:PureWP a) (p:PurePost a) -> wp (fun a -> p a)
+// // // sub_effect
+// // //   DIV   ~> EXN   = fun (a:Type) (wp:PureWP a) (p:ExPost a) -> wp (fun a -> p (V a))
 
-type lex_t =
-  | LexTop  : lex_t
-  | LexCons : #a:Type -> a -> lex_t -> lex_t
+// // // type lex_t =
+// // //   | LexTop  : lex_t
+// // //   | LexCons : #a:Type -> a -> lex_t -> lex_t
 
-type Tuple2 'a 'b =
-  | MkTuple2: _1:'a
-           -> _2:'b
-           -> Tuple2 'a 'b
+// // // type Tuple2 'a 'b =
+// // //   | MkTuple2: _1:'a
+// // //            -> _2:'b
+// // //            -> Tuple2 'a 'b
 
-type Tuple3 'a 'b 'c =
-  | MkTuple3: _1:'a
-           -> _2:'b
-           -> _3:'c
-          -> Tuple3 'a 'b 'c
+// // // type Tuple3 'a 'b 'c =
+// // //   | MkTuple3: _1:'a
+// // //            -> _2:'b
+// // //            -> _3:'c
+// // //           -> Tuple3 'a 'b 'c
 
-type Tuple4 'a 'b 'c 'd =
-  | MkTuple4: _1:'a
-           -> _2:'b
-           -> _3:'c
-           -> _4:'d
-           -> Tuple4 'a 'b 'c 'd
+// // // type Tuple4 'a 'b 'c 'd =
+// // //   | MkTuple4: _1:'a
+// // //            -> _2:'b
+// // //            -> _3:'c
+// // //            -> _4:'d
+// // //            -> Tuple4 'a 'b 'c 'd
 
-type Tuple5 'a 'b 'c 'd 'e =
-  | MkTuple5: _1:'a
-           -> _2:'b
-           -> _3:'c
-           -> _4:'d
-           -> _5:'e
-           -> Tuple5 'a 'b 'c 'd 'e
+// // // type Tuple5 'a 'b 'c 'd 'e =
+// // //   | MkTuple5: _1:'a
+// // //            -> _2:'b
+// // //            -> _3:'c
+// // //            -> _4:'d
+// // //            -> _5:'e
+// // //            -> Tuple5 'a 'b 'c 'd 'e
 
-type Tuple6 'a 'b 'c 'd 'e 'f =
-  | MkTuple6: _1:'a
-           -> _2:'b
-           -> _3:'c
-           -> _4:'d
-           -> _5:'e
-           -> _6:'f
-           -> Tuple6 'a 'b 'c 'd 'e 'f
-
-
-type Tuple7 'a 'b 'c 'd 'e 'f 'g =
-  | MkTuple7: _1:'a
-           -> _2:'b
-           -> _3:'c
-           -> _4:'d
-           -> _5:'e
-           -> _6:'f
-           -> _7:'g
-           -> Tuple7 'a 'b 'c 'd 'e 'f 'g
+// // // type Tuple6 'a 'b 'c 'd 'e 'f =
+// // //   | MkTuple6: _1:'a
+// // //            -> _2:'b
+// // //            -> _3:'c
+// // //            -> _4:'d
+// // //            -> _5:'e
+// // //            -> _6:'f
+// // //            -> Tuple6 'a 'b 'c 'd 'e 'f
 
 
-type Tuple8 'a 'b 'c 'd 'e 'f 'g 'h =
-  | MkTuple8: _1:'a
-           -> _2:'b
-           -> _3:'c
-           -> _4:'d
-           -> _5:'e
-           -> _6:'f
-           -> _7:'g
-           -> _8:'h
-           -> Tuple8 'a 'b 'c 'd 'e 'f 'g 'h
-
-// type DTuple3 (a:Type)
-//              (b:(a -> Type))
-//              (c:(x:a -> b x -> Type)) =
-//    | MkDTuple3:_1:a
-//              -> _2:b _1
-//              -> _3:c _1 _2
-//              -> DTuple3 a b c
-
-// type DTuple4 (a:Type)
-//              (b:(x:a -> Type))
-//              (c:(x:a -> b x -> Type))
-//              (d:(x:a -> y:b x -> z:c x y -> Type)) =
-//  | MkDTuple4:_1:a
-//            -> _2:b _1
-//            -> _3:c _1 _2
-//            -> _4:d _1 _2 _3
-//            -> DTuple4 a b c d
+// // // type Tuple7 'a 'b 'c 'd 'e 'f 'g =
+// // //   | MkTuple7: _1:'a
+// // //            -> _2:'b
+// // //            -> _3:'c
+// // //            -> _4:'d
+// // //            -> _5:'e
+// // //            -> _6:'f
+// // //            -> _7:'g
+// // //            -> Tuple7 'a 'b 'c 'd 'e 'f 'g
 
 
-type as_requires (#a:Type) (wp:PureWP a)  = wp (fun x -> True)
-type as_ensures  (#a:Type) (wlp:PureWP a) (x:a) = ~ (wlp (fun y -> (y=!=x)))
+// // // type Tuple8 'a 'b 'c 'd 'e 'f 'g 'h =
+// // //   | MkTuple8: _1:'a
+// // //            -> _2:'b
+// // //            -> _3:'c
+// // //            -> _4:'d
+// // //            -> _5:'e
+// // //            -> _6:'f
+// // //            -> _7:'g
+// // //            -> _8:'h
+// // //            -> Tuple8 'a 'b 'c 'd 'e 'f 'g 'h
 
-// val fst : ('a * 'b) -> Tot 'a
-// let fst x = MkTuple2._1 x
+// // // type DTuple3 (a:Type)
+// // //              (b:(a -> Type))
+// // //              (c:(x:a -> b x -> Type)) =
+// // //    | MkDTuple3:_1:a
+// // //              -> _2:b _1
+// // //              -> _3:c _1 _2
+// // //              -> DTuple3 a b c
 
+// // // type DTuple4 (a:Type)
+// // //              (b:(x:a -> Type))
+// // //              (c:(x:a -> b x -> Type))
+// // //              (d:(x:a -> y:b x -> z:c x y -> Type)) =
+// // //  | MkDTuple4:_1:a
+// // //            -> _2:b _1
+// // //            -> _3:c _1 _2
+// // //            -> _4:d _1 _2 _3
+// // //            -> DTuple4 a b c d
 
-// val snd : ('a * 'b) -> Tot 'b
-// let snd x = MkTuple2._2 x
+// // // type as_requires (#a:Type) (wp:PureWP a)  = wp (fun x -> True)
+// // // type as_ensures  (#a:Type) (wlp:PureWP a) (x:a) = ~ (wlp (fun y -> (y=!=x)))
 
-// val dfst : #a:Type -> #b:(a -> Type) -> DTuple2 a b -> Tot a
-// let dfst #a #b t = MkDTuple2._1 t
+// // // // val fst : ('a * 'b) -> Tot 'a
+// // // // let fst x = MkTuple2._1 x
 
-// val dsnd : #a:Type -> #b:(a -> Type) -> t:(DTuple2 a b) -> Tot (b (MkDTuple2._1 t))
-// let dsnd #a #b t = MkDTuple2._2 t
+// // // // val snd : ('a * 'b) -> Tot 'b
+// // // // let snd x = MkTuple2._2 x
 
-type Let (#a:Type) (x:a) (body:(a -> Type)) = body x
-logic type InductionHyp : #a:Type -> a -> Type -> Type
-assume val by_induction_on: #a:Type -> #p:Type -> induction_on:a -> proving:p -> Lemma (ensures (InductionHyp induction_on p))
-logic type Using : #a:Type -> Type -> a -> Type
-assume val using: #a:Type -> #p:Type -> proving:p -> pat:a -> Lemma (ensures (Using p pat))
-assume val _assume : p:Type -> unit -> Pure unit (requires (True)) (ensures (fun x -> p))
-assume val admit   : #a:Type -> unit -> Admit a
-assume val magic   : #a:Type -> unit -> Tot a
-assume val admitP  : p:Type -> Pure unit True (fun x -> p)
-assume val _assert : p:Type -> unit -> Pure unit (requires $"assertion failed" p) (ensures (fun x -> True))
-assume val cut     : p:Type -> Pure unit (requires $"assertion failed" p) (fun x -> p)
-assume val qintro  : #a:Type -> #p:(a -> Type) -> =f:(x:a -> Lemma (p x)) -> Lemma (forall (x:a). p x)
-assume val ghost_lemma: #a:Type -> #p:(a -> Type) -> #q:(a -> unit -> Type) -> =f:(x:a -> Ghost unit (p x) (q x)) -> Lemma (forall (x:a). p x ==> q x ())
-assume val raise: exn -> Ex 'a       (* TODO: refine with the Exn monad *)
-val ignore: #a:Type -> a -> Tot unit
-let ignore #a x = ()
+// // // // val dfst : #a:Type -> #b:(a -> Type) -> DTuple2 a b -> Tot a
+// // // // let dfst #a #b t = MkDTuple2._1 t
 
-(* type nat = i:int{i >= 0} *)
-(* type pos = i:int{i > 0} *)
-(* type nonzero = i:int{i<>0} *)
+// // // // val dsnd : #a:Type -> #b:(a -> Type) -> t:(DTuple2 a b) -> Tot (b (MkDTuple2._1 t))
+// // // // let dsnd #a #b t = MkDTuple2._2 t
 
-(* (\* For the moment we require not just that the divisor is non-zero, *)
-(*    but also that the dividend is natural. This works around a *)
-(*    mismatch between the semantics of integer division in SMT-LIB and *)
-(*    in F#/OCaml. For SMT-LIB ints the modulus is always positive (as in *)
-(*    math Euclidian division), while for F#/OCaml ints the modulus has *)
-(*    the same sign as the dividend. Our arbitrary precision ints don't *)
-(*    quite correspond to finite precision F#/OCaml ints though, but to *)
-(*    OCaml's big_ints (for which the modulus is always positive).  So *)
-(*    we'll need to return to this point anyway, when we discuss how to *)
-(*    soundly map F* ints to something in F#/OCaml. *\) *)
-(* assume val op_Modulus            : int -> nonzero -> Tot int *)
-(* assume val op_Division           : nat -> nonzero -> Tot int *)
+// // // type Let (#a:Type) (x:a) (body:(a -> Type)) = body x
+// // // logic type InductionHyp : #a:Type -> a -> Type -> Type
+// // // assume val by_induction_on: #a:Type -> #p:Type -> induction_on:a -> proving:p -> Lemma (ensures (InductionHyp induction_on p))
+// // // logic type Using : #a:Type -> Type -> a -> Type
+// // // assume val using: #a:Type -> #p:Type -> proving:p -> pat:a -> Lemma (ensures (Using p pat))
+// // // assume val _assume : p:Type -> unit -> Pure unit (requires (True)) (ensures (fun x -> p))
+// // // assume val admit   : #a:Type -> unit -> Admit a
+// // // assume val magic   : #a:Type -> unit -> Tot a
+// // // assume val admitP  : p:Type -> Pure unit True (fun x -> p)
+// // // assume val _assert : p:Type -> unit -> Pure unit (requires $"assertion failed" p) (ensures (fun x -> True))
+// // // assume val cut     : p:Type -> Pure unit (requires $"assertion failed" p) (fun x -> p)
+// // // assume val qintro  : #a:Type -> #p:(a -> Type) -> =f:(x:a -> Lemma (p x)) -> Lemma (forall (x:a). p x)
+// // // assume val ghost_lemma: #a:Type -> #p:(a -> Type) -> #q:(a -> unit -> Type) -> =f:(x:a -> Ghost unit (p x) (q x)) -> Lemma (forall (x:a). p x ==> q x ())
+// // // assume val raise: exn -> Ex 'a       (* TODO: refine with the Exn monad *)
+// // // val ignore: #a:Type -> a -> Tot unit
+// // // let ignore #a x = ()
 
-assume val string_of_bool: bool -> Tot string
-assume val string_of_int: int -> Tot string
+// // // (* type nat = i:int{i >= 0} *)
+// // // (* type pos = i:int{i > 0} *)
+// // // (* type nonzero = i:int{i<>0} *)
+
+// // // (*    For the moment we require not just that the divisor is non-zero, *)
+// // // (*    but also that the dividend is natural. This works around a *)
+// // // (*    mismatch between the semantics of integer division in SMT-LIB and *)
+// // // (*    in F#/OCaml. For SMT-LIB ints the modulus is always positive (as in *)
+// // // (*    math Euclidian division), while for F#/OCaml ints the modulus has *)
+// // // (*    the same sign as the dividend. Our arbitrary precision ints don't *)
+// // // (*    quite correspond to finite precision F#/OCaml ints though, but to *)
+// // // (*    OCaml's big_ints (for which the modulus is always positive).  So *)
+// // // (*    we'll need to return to this point anyway, when we discuss how to *)
+// // // (*    soundly map F* ints to something in F#/OCaml.  *)
+
+// // // (* assume val op_Modulus            : int -> nonzero -> Tot int *)
+// // // (* assume val op_Division           : nat -> nonzero -> Tot int *)
+
+// // // assume val string_of_bool: bool -> Tot string
+// // // assume val string_of_int: int -> Tot string
